pulse/lib/pulse/core/PulseCore.Memory.fsti
@@ -201,12 +201,19 @@ let _PST
         interp (provides x `star` frame `star` locks_invariant except m1) m1)
 
 (** An action is just a thunked computation in [MstTot] that takes a frame as argument *)
-let action_except (a:Type u#a) (except:inames) (expects:slprop) (provides: a -> slprop) =
+let action_except (a:Type u#a) (except:inames) (expects:slprop) (provides: a -> slprop)
+  : Type u#(max a 2) =
   frame:slprop -> MstTot a except expects provides frame
 
 (** An action is just a thunked computation in [MstTot] that takes a frame as argument *)
-let _pst_action_except (a:Type u#a) (maybe_ghost:bool) (except:inames) (expects:slprop) (provides: a -> slprop) =
-  frame:slprop -> _PST a maybe_ghost except expects provides frame
+let _pst_action_except 
+    (a:Type u#a)
+    (maybe_ghost:bool)
+    (except:inames)
+    (expects:slprop)
+    (provides: a -> slprop)
+ : Type u#(max a 2) 
+ = frame:slprop -> _PST a maybe_ghost except expects provides frame
 
 let pst_action_except (a:Type u#a) (except:inames) (expects:slprop) (provides: a -> slprop) =
   _pst_action_except a false except expects provides
@@ -405,3 +412,75 @@ val intro_pure (#opened_invariants:_) (p:prop) (_:squash p)
 
 val drop (#opened_invariants:_) (p:slprop)
   : pst_ghost_action_except unit opened_invariants p (fun _ -> emp)
+
+let non_info a = x:erased a -> y:a { reveal x == y}
+val lift_ghost
+      (#a:Type)
+      #opened_invariants #p #q
+      (ni_a:non_info a)
+      (f:erased (pst_ghost_action_except a opened_invariants p q))
+  : pst_ghost_action_except a opened_invariants p q
+
+[@@erasable]
+val ghost_ref (#[@@@unused] a:Type u#a) ([@@@unused]p:pcm a) : Type0
+val ghost_pts_to (#a:Type u#a) (#p:pcm a) (r:ghost_ref p) (v:a) : slprop u#a
+
+val ghost_alloc
+    (#o:_)
+    (#a:Type u#1)
+    (#pcm:pcm a)
+    (x:erased a{compatible pcm x x /\ pcm.refine x})
+: pst_ghost_action_except
+    (ghost_ref pcm)
+    o
+    emp 
+    (fun r -> ghost_pts_to r x)
+
+val ghost_read
+    #o
+    (#a:Type)
+    (#p:pcm a)
+    (r:ghost_ref p)
+    (x:erased a)
+    (f:(v:a{compatible p x v}
+        -> GTot (y:a{compatible p y v /\
+                     FStar.PCM.frame_compatible p x v y})))
+: pst_ghost_action_except
+    (erased (v:a{compatible p x v /\ p.refine v}))
+    o
+    (ghost_pts_to r x)
+    (fun v -> ghost_pts_to r (f v))
+
+val ghost_write
+    #o
+    (#a:Type)
+    (#p:pcm a)
+    (r:ghost_ref p)
+    (x y:Ghost.erased a)
+    (f:FStar.PCM.frame_preserving_upd p x y)
+: pst_ghost_action_except unit o 
+    (ghost_pts_to r x)
+    (fun _ -> ghost_pts_to r y)
+
+val ghost_share
+    #o
+    (#a:Type)
+    (#pcm:pcm a)
+    (r:ghost_ref pcm)
+    (v0:FStar.Ghost.erased a)
+    (v1:FStar.Ghost.erased a{composable pcm v0 v1})
+: pst_ghost_action_except unit o
+    (ghost_pts_to r (v0 `op pcm` v1))
+    (fun _ -> ghost_pts_to r v0 `star` ghost_pts_to r v1)
+
+val ghost_gather
+    #o
+    (#a:Type)
+    (#pcm:pcm a)
+    (r:ghost_ref pcm)
+    (v0:FStar.Ghost.erased a)
+    (v1:FStar.Ghost.erased a)
+: pst_ghost_action_except
+    (squash (composable pcm v0 v1)) o
+    (ghost_pts_to r v0 `star` ghost_pts_to r v1)
+    (fun _ -> ghost_pts_to r (op pcm v0 v1))
